src/CvmSemantics.v
@@ -2068,14 +2068,8 @@ Proof.
 Defined.
 
 
-Axiom events_cvm_to_core : forall t p e,
-    cvm_events t p e = cvm_events_core (term_to_core_term t) p e.
-
 Axiom events_cvm_to_core_mt : forall t p e,
     cvm_events_core (lseqc (aspc CLEAR) t) p e = cvm_events_core t p mt.
-
-Axiom evidence_cvm_to_core : forall t p e,
-    cvm_evidence t p e = cvm_evidence_core (term_to_core_term t) p e.
 
 Axiom ev_cvm_mtc: forall ct p e loc,
     parallel_vm_thread loc ct p mt_evc = parallel_vm_thread loc (lseqc (aspc CLEAR) ct) p e.
@@ -2250,7 +2244,7 @@ Proof.
     assert (evc bits' et' = cvm_evidence_core (term_to_core_term t') p (evc bits et)). {
 
       rewrite at_evidence in *.
-      rewrite evidence_cvm_to_core in *.
+      unfold cvm_evidence in *.
       rewrite H5.
       tauto.
     }
@@ -2723,7 +2717,7 @@ Proof.
 
     rewrite par_evidence in *.
 
-    rewrite evidence_cvm_to_core in *.
+    unfold cvm_evidence in *.
     rewrite Heqe0 in *.
 
 
@@ -2826,7 +2820,7 @@ Axiom evidence_cvm_to_core : forall t p e,
 
     rewrite par_evidence in *.
 
-    rewrite evidence_cvm_to_core in *.
+    unfold cvm_evidence in *.
     rewrite Heqe0 in *.
 
 
@@ -2934,7 +2928,7 @@ Axiom evidence_cvm_to_core : forall t p e,
 
     rewrite par_evidence in *.
 
-    rewrite evidence_cvm_to_core in *.
+    unfold cvm_evidence in *.
     rewrite Heqe0 in *.
 
 
@@ -3031,19 +3025,11 @@ Axiom evidence_cvm_to_core : forall t p e,
 
     wrap_ccp_anno.
 
-
-    (*
-Axiom evidence_cvm_to_core : forall t p e,
-    cvm_evidence t p e = cvm_evidence_core (term_to_core_term t) p e.
-     *)
-
-    
-
     rewrite <- ev_cvm_mtc in *.
 
     rewrite par_evidence in *.
 
-    rewrite evidence_cvm_to_core in *.
+    unfold cvm_evidence in *.
     rewrite Heqe0 in *.
 
 
@@ -3735,7 +3721,7 @@ Proof.
       
       eapply lstar_transitive.
 
-      rewrite <- events_cvm_to_core.
+      unfold cvm_events in *.
       
       eapply bpar_shuffle.
       eassumption.
@@ -3827,7 +3813,7 @@ Proof.
       
       eapply lstar_transitive.
 
-      rewrite <- events_cvm_to_core.
+      unfold cvm_events in *.
       
       eapply bpar_shuffle.
       eassumption.
@@ -3921,7 +3907,7 @@ Proof.
       
       eapply lstar_transitive.
 
-      rewrite <- events_cvm_to_core.
+      unfold cvm_events in *.
       
       eapply bpar_shuffle.
       eassumption.
@@ -4014,7 +4000,7 @@ Proof.
       
       eapply lstar_transitive.
 
-      rewrite <- events_cvm_to_core.
+      unfold cvm_events in *.
       
       eapply bpar_shuffle.
       eassumption.
